---
title: "Assignment 1"
author: "Qianlang Chen"

date: "Mon 01/13/2020"
output: pdf_document
---

```{r setup, include=FALSE}
knitr::opts_chunk$set(echo = TRUE)
```

# Section 1.2

### Exercise 1.m (p21)

(todo)

### Exercise 7.g (p21)

First five terms:

* $a_1=2^{2\times1-1}-1=1$

* $a_2=2^{2\times2-1}-1=7$

* $a_3=2^{2\times3-1}-1=31$

* $a_4=2^{2\times4-1}-1=127$

* $a_5=2^{2\times5-1}-1=511$

Recursive formula:

$$a_1=1;a_n=4\times a_{n-1}+3$$

### Exercise 9.a (p21)

First five terms:

* $a_1=5$

* $a_2=a_{2-1}+(2+4)=11$

* $a_3=a_{3-1}+(3+4)=18$

* $a_4=a_{4-1}+(4+4)=26$

* $a_5=a_{5-1}+(5+4)=35$

Closed formula:

$$a_n=\frac{n^2+n}{2}+4n$$

### Exercise 30 (p23)

**Part (a)**

* $a_1=A$

* $a_2=a_{2/2}B=a_1B=AB$

* $a_3=a_{(3-1)/2}A=a_1A=AA$

* $a_4=a_{4/2}B=a_2B=ABB$

* $a_5=a_{(5-1)/2}A=a_2A=ABA$

* $a_6=a_{6/2}B=a_3B=AAB$

* $a_7=a_{(7-1)/2}A=a_3A=AAA$

* $a_8=a_{8/2}B=a_4B=ABBB$

* $a_9=a_{(9-1)/2}A=a_4A=ABBA$

* $a_{10}=a_{10/2}B=a_5B=ABAB$

**Part (b)**

* $a_{17}=a_{(17-1)/2}A=a_8A=ABBBA$

* $a_{21}=a_{(21-1)/2}A=a_{10}A=ABABA$

**Part (c)**

* $a_{630}=a_{630/2}B=a_{315}B=ABBAAABAAB$

* $a_{631}=a_{(631-1)/2}A=a_{315}A=ABBAAABAAA$

\pagebreak
# Section 1.3

### Exercise 1.a (p37)

Let $p$ represent "$A$ is telling the truth" and $q$ represent "$B$ is telling the truth," according to the information given by the problem, we can generate the following truth table:

|$p$|$q$|$p\land q$|$\lnot p$|
|:-:|:-:|:--------:|:-------:|
|T  |T  |T         |F        |
|T  |F  |T         |T        |
|F  |T  |F         |T        |
|F  |F  |F         |T        |

As seen from the truth table, only the third row provides a consistent result (where when $p=F$ and $q=T$, $p=p\land q$ and $q=\lnot p$). Therefore, $A$ is lying, and $B$ is telling the truth.

### Exercise 4.a (p37)

$$\lnot p\land(q\lor r)$$

where $p$, $q$, and $r$ represent $A$, $B$, and $C$ being truthful, respectively.

### Exercise 10.d (p38)

$$(x\leq0)\land(y\leq0)$$

### Exercise 24.b (p40)

\begin{align}
(p\lor t)\land(p\lor c)&\equiv t\land(p\lor c)&\text{Universal bound}
&\equiv t\land p&\text{Identity}
&\equiv p\land t&\text{Commutative}
&\equiv p&\text{Identity}
\end{align}

### Problem 7 (Java method)

Since `charIsNotLowerCaseLetter(c)` always produces exactly the opposite result of `charIsLowerCaseLetter(c)` and the definition of `charIsLowerCaseLetter(c)` is `'a' <= c && c <= 'z'`, according to DeMorgan's Law,

```
!('a' <= c && c <= 'z')
=== !('a' <= c) || !(c <= 'z')
=== 'a' > c || c > 'z'
```

\pagebreak
# Section 1.4

### Exercise 14.c (p52)



### Exercise 15.c (p52)



### Exercise 17.c (p52)



### Exercise 20.b (p52)



\pagebreak
# Section 1.5

### Exercise 11.c (p66)



### Exercise 11.e (p66)



### Exercise 14.d (p67)



### Exercise 17.a (p67)



### Exercise 25.e (p67)



### Exercise 26.e (p67)



### Exercise 27.e (p67)





















